src/lang/Event.v
@@ -19,65 +19,18 @@ Module LocMap := IdentMap.
 Module LocFun := IdentFun.
 
 
-Module Const <: OrderedTypeWithLeibniz.
-  Include Nat.
-
-  Lemma eq_leibniz (x y: t): eq x y -> x = y.
-  Proof. auto. Qed.
-
-  Ltac ltb_tac :=
-    match goal with
-    | [H: compare ?x1 ?x2 = _ |- _] =>
-      generalize (compare_spec x1 x2); rewrite H; clear H;
-      intro H; inversion H; subst; clear H
-    | [H: lt ?x ?x |- _] =>
-      destruct lt_strorder; congruence
-    | [H: lt ?x ?y |- _] =>
-      rewrite H in *; clear H
-    | [H: eq ?x ?y |- _] =>
-      rewrite H in *; clear H
-    end.
-End Const.
+Module Const := Nat.
 
 
-Module Ordering <: OrderedTypeWithLeibniz.
-  Module Raw <: BoolOrderedType.S.
-    Inductive t_ :=
-    | relaxed
-    | acquire
-    | release
-    | relacq
-    .
-    Definition t := t_.
-
-    Definition eq_dec (x y:t): {x = y} + {x <> y}.
-    Proof. decide equality. Qed.
-
-    Definition ltb (lhs rhs:t): bool :=
-      match lhs, rhs with
-      | relaxed, relaxed => false
-      | relaxed, _ => true
-      | acquire, relaxed => false
-      | acquire, acquire => false
-      | acquire, _ => true
-      | release, relaxed => false
-      | release, acquire => false
-      | release, release => false
-      | release, _ => true
-      | relacq, _ => false
-      end.
-
-    Lemma ltb_trans (x y z:t) (XY: ltb x y) (YZ: ltb y z): ltb x z.
-    Proof. repeat intro. destruct x, y, z; auto. Qed.
-
-    Lemma ltb_irrefl x: ~ ltb x x.
-    Proof. repeat intro. destruct x; auto. Qed.
-
-    Lemma ltb_eq (lhs rhs:t) (LR: ~ ltb lhs rhs) (RL: ~ ltb rhs lhs): lhs = rhs.
-    Proof. repeat intro. destruct lhs, rhs; simpl in *; congruence. Qed.
-  End Raw.
-
-  Include Raw <+ BoolOrderedType.Make (Raw).
+Module Ordering.
+  (* TODO: support the unordered/monotonic atomics (#46) *)
+  (* TODO: support the SC atomics (#40) *)
+  Inductive t :=
+  | relaxed
+  | acquire
+  | release
+  | relacq
+  .
 
   Definition ord (lhs rhs:t): bool :=
     match lhs, rhs with
@@ -90,81 +43,20 @@ Module Ordering <: OrderedTypeWithLeibniz.
 End Ordering.
 
 
-Module RWEvent <: OrderedTypeWithLeibniz.
-  Module Raw <: BoolOrderedType.S.
-    Inductive t_ :=
-    | read (loc:Loc.t) (val:Const.t) (ord:Ordering.t)
-    | write (loc:Loc.t) (val:Const.t) (ord:Ordering.t)
-    | update (loc:Loc.t) (rval wval:Const.t) (ord:Ordering.t)
-    .
-    Definition t := t_.
-
-    Definition eq_dec (x y:t): {x = y} + {x <> y}.
-    Proof.
-      decide equality;
-        (try apply Loc.eq_dec);
-        (try apply Const.eq_dec);
-        (try apply Ordering.eq_dec).
-    Qed.
-
-    Definition ltb (lhs rhs:t): bool :=
-      match lhs, rhs with
-      | read l1 v1 o1, read l2 v2 o2 =>
-        compose_comparisons [Loc.compare l1 l2; Const.compare v1 v2; Ordering.compare o1 o2]
-      | write l1 v1 o1, write l2 v2 o2 =>
-        compose_comparisons [Loc.compare l1 l2; Const.compare v1 v2; Ordering.compare o1 o2]
-      | update l1 r1 w1 o1, update l2 r2 w2 o2 =>
-        compose_comparisons [Loc.compare l1 l2; Const.compare r1 r2; Const.compare w1 w2; Ordering.compare o1 o2]
-      | read _ _ _, _ => true
-      | write _ _ _, read _ _ _ => false
-      | write _ _ _, _ => true
-      | update _ _ _ _, _ => false
-      end.
-
-    Lemma ltb_trans (x y z:t) (XY: ltb x y) (YZ: ltb y z): ltb x z.
-    Proof.
-      destruct x, y, z; simpl in *; auto;
-        repeat
-          (try congruence;
-           try omega;
-           try Loc.ltb_tac;
-           try Const.ltb_tac;
-           try Ordering.ltb_tac;
-           try ltb_des).
-    Qed.
-
-    Lemma ltb_irrefl x: ~ ltb x x.
-    Proof.
-      destruct x; simpl in *; auto;
-        repeat
-          (try congruence;
-           try omega;
-           try Loc.ltb_tac;
-           try Const.ltb_tac;
-           try Ordering.ltb_tac;
-           try ltb_des).
-    Qed.
-
-    Lemma ltb_eq (lhs rhs:t) (LR: ~ ltb lhs rhs) (RL: ~ ltb rhs lhs): lhs = rhs.
-    Proof.
-      destruct lhs, rhs; simpl in *; auto;
-        repeat
-          (try congruence;
-           try omega;
-           try Loc.ltb_tac;
-           try Const.ltb_tac;
-           try Ordering.ltb_tac;
-           try ltb_des).
-    Qed.
-  End Raw.
-
-  Include Raw <+ BoolOrderedType.Make (Raw).
+Module MemEvent.
+  Inductive t :=
+  | read (loc:Loc.t) (val:Const.t) (ord:Ordering.t)
+  | write (loc:Loc.t) (val:Const.t) (ord:Ordering.t)
+  | update (loc:Loc.t) (rval wval:Const.t) (ord:Ordering.t)
+  | fence (ord:Ordering.t)
+  .
 
   Definition is_writing (e:t): option (Loc.t * Const.t * Ordering.t) :=
     match e with
     | read _ _ _ => None
     | write loc val ord => Some (loc, val, ord)
     | update loc _ val ord => Some (loc, val, ord)
+    | fence _ => None
     end.
 
   Definition is_writing_to (loc:Loc.t) (e:t): option(Const.t * Ordering.t) :=
@@ -181,6 +73,7 @@ Module RWEvent <: OrderedTypeWithLeibniz.
     | read loc val ord => Some (loc, val, ord)
     | write _ _ _ => None
     | update loc val _ ord => Some (loc, val, ord)
+    | fence _ => None
     end.
 
   Definition get_ordering (e:t): Ordering.t :=
@@ -188,42 +81,22 @@ Module RWEvent <: OrderedTypeWithLeibniz.
     | read _ _ ord => ord
     | write _ _ ord => ord
     | update _ _ _ ord => ord
+    | fence ord => ord
     end.
-
-  Definition is_inceptionable (e:t): bool :=
-    if is_writing e
-    then negb (Ordering.ord Ordering.release (get_ordering e))
-    else false.
-End RWEvent.
+End MemEvent.
 
 
 Module Event.
-  Structure t_ := mk {
+  Structure t := mk {
     lhs: Const.t;
     rhses: list Const.t;
   }.
-  Definition t := t_.
-
-  Definition eq := @eq t.
-  Program Instance eq_equiv: Equivalence eq.
-  Definition eq_dec (x y:t): {eq x y} + {~ eq x y}.
-  Proof.
-    unfold eq.
-    decide equality;
-      (try apply list_eq_dec);
-      (try apply Const.eq_dec).
-  Qed.
 End Event.
 
 
 Module ThreadEvent.
-  Inductive mem_t :=
-  | rw (e:RWEvent.t)
-  | fence (ord:Ordering.t)
-  .
-
   Inductive t :=
-  | mem (e:mem_t)
+  | mem (e:MemEvent.t)
   | syscall (e:Event.t)
   .
 End ThreadEvent.
